<?xml version="1.0" encoding="UTF-8"?>
<rdf:RDF
   xmlns:adms="http://www.w3.org/ns/adms#"
   xmlns:clvapit="https://w3id.org/italia/onto/CLV/"
   xmlns:dcat="http://www.w3.org/ns/dcat#"
   xmlns:dct="http://purl.org/dc/terms/"
   xmlns:foaf="http://xmlns.com/foaf/0.1/"
   xmlns:owl="http://www.w3.org/2002/07/owl#"
   xmlns:rdf="http://www.w3.org/1999/02/22-rdf-syntax-ns#"
   xmlns:rdfs="http://www.w3.org/2000/01/rdf-schema#"
   xmlns:skos="http://www.w3.org/2004/02/skos/core#"
   xmlns:vcard="http://www.w3.org/2006/vcard/ns#"
   xmlns:xkos="http://rdf-vocabulary.ddialliance.org/xkos#"
>
  <rdf:Description rdf:about="http://dati.gov.it/data/resource/Distribution/LE_RDF_XML">
    <dct:license rdf:resource="https://w3id.org/italia/controlled-vocabulary/licences/A21_CCBY40"/>
    <dcat:downloadURL rdf:resource="https://raw.githubusercontent.com/italia/dati-semantic-assets/master/VocabolariControllati/classifications-for-public-services/life-busines-event/life-event/life-event.rdf"/>
    <rdf:type rdf:resource="http://dati.gov.it/onto/dcatapit#Distribution"/>
    <dct:format rdf:resource="http://publications.europa.eu/resource/authority/file-type/RDF_XML"/>
    <dct:title xml:lang="it">Distribuzione RDF/XML eventi della vita</dct:title>
    <dct:description xml:lang="en">This is the distribution in RDF/XML of the Linked Open Dataset of the controlled vocabulary related to the life events used in the Italian national catalogue of public services</dct:description>
    <dcat:accessURL rdf:resource="https://raw.githubusercontent.com/italia/dati-semantic-assets/master/VocabolariControllati/classifications-for-public-services/life-busines-event/life-event"/>
    <dct:title xml:lang="en">RDF/XML distribution life events</dct:title>
    <dct:description xml:lang="it">Questa è la distribuzione RDF/XML del dataset Linked Open Data del vocabolario controllato sulla classificazione degli eventi della vita usati nel catalogo nazionale per i servizi pubblici</dct:description>
  </rdf:Description>
  <rdf:Description rdf:about="https://w3id.org/italia/controlled-vocabulary/classifications-for-public-services/life-business-event/life-event/18">
    <skos:prefLabel xml:lang="de">Zugang zu öffentlichen Kulturstätten</skos:prefLabel>
    <skos:definition xml:lang="en">This life event groups public services related to the access to public cultural sites such as the payment of a ticket or the use of public library</skos:definition>
    <rdf:type rdf:resource="http://www.w3.org/2004/02/skos/core#Concept"/>
    <rdf:type rdf:resource="https://w3id.org/italia/onto/CPSV/LifeEvent"/>
    <skos:prefLabel xml:lang="en">Access to public cultural sites</skos:prefLabel>
    <skos:prefLabel xml:lang="it">Accesso luoghi della cultura</skos:prefLabel>
    <skos:inScheme rdf:resource="https://w3id.org/italia/controlled-vocabulary/classifications-for-public-services/life-business-event/life-event"/>
    <skos:notation>18</skos:notation>
    <clvapit:hasRankOrder>1</clvapit:hasRankOrder>
    <dct:identifier>18</dct:identifier>
    <skos:definition xml:lang="it">Questo evento della vita raggruppa servizi pubblici relativi all'accesso ai luoghi della cultura pubblici come per esempio il pagamento di un biglietto di entrata, o l'uso di una biblioteca pubblica</skos:definition>
  </rdf:Description>
  <rdf:Description rdf:about="https://w3id.org/italia/controlled-vocabulary/classifications-for-public-services/life-business-event/life-event/2">
    <skos:definition xml:lang="en">This life event groups public services related to a severe health problem, for instance getting disabled.</skos:definition>
    <skos:prefLabel xml:lang="en">Disability</skos:prefLabel>
    <skos:inScheme rdf:resource="https://w3id.org/italia/controlled-vocabulary/classifications-for-public-services/life-business-event/life-event"/>
    <clvapit:hasRankOrder>1</clvapit:hasRankOrder>
    <skos:prefLabel xml:lang="it">Invalidità</skos:prefLabel>
    <rdf:type rdf:resource="http://www.w3.org/2004/02/skos/core#Concept"/>
    <skos:definition xml:lang="it">Questo evento della vita raggruppa servizi pubblici relativi a seri problemi di salute come per esempio diventare disabile</skos:definition>
    <dct:identifier>2</dct:identifier>
    <skos:notation>2</skos:notation>
    <skos:prefLabel xml:lang="de">Behinderung / Unfähigkeit</skos:prefLabel>
    <rdf:type rdf:resource="https://w3id.org/italia/onto/CPSV/LifeEvent"/>
  </rdf:Description>
  <rdf:Description rdf:about="https://w3id.org/italia/controlled-vocabulary/classifications-for-public-services/life-business-event/life-event/10">
    <skos:prefLabel xml:lang="it">Espatrio per lavoro, studio, pensionamento</skos:prefLabel>
    <skos:definition xml:lang="it">Questo evento della vita raggruppa servizi pubblici relativi a quando qualcuno espatria (per diversi motivi che possono riguardare: il lavoro, lo studio, il pensionamento)</skos:definition>
    <rdf:type rdf:resource="https://w3id.org/italia/onto/CPSV/LifeEvent"/>
    <skos:definition xml:lang="en">This life event groups public services that relate to when someone moves from one country to another.</skos:definition>
    <clvapit:hasRankOrder>1</clvapit:hasRankOrder>
    <skos:prefLabel xml:lang="de">Umzug oder Vorbereitung auf den Umzug in ein anderes Land (z. B. um zu studieren, arbeiten, in Rente gehen, ...)</skos:prefLabel>
    <dct:identifier>10</dct:identifier>
    <skos:inScheme rdf:resource="https://w3id.org/italia/controlled-vocabulary/classifications-for-public-services/life-business-event/life-event"/>
    <skos:notation>10</skos:notation>
    <rdf:type rdf:resource="http://www.w3.org/2004/02/skos/core#Concept"/>
    <skos:prefLabel xml:lang="en">Moving or preparing to move to another country (e.g., to study, work, retire, ..)</skos:prefLabel>
  </rdf:Description>
  <rdf:Description rdf:about="https://w3id.org/italia/controlled-vocabulary/classifications-for-public-services/life-business-event/life-event/9">
    <skos:prefLabel xml:lang="de">Wohnortwechsel/Domizilwechsel innerhalb eines Landes</skos:prefLabel>
    <rdf:type rdf:resource="https://w3id.org/italia/onto/CPSV/LifeEvent"/>
    <skos:prefLabel xml:lang="en">Moving and changing address within one country</skos:prefLabel>
    <skos:notation>9</skos:notation>
    <skos:prefLabel xml:lang="it">Cambio di residenza/domicilio</skos:prefLabel>
    <skos:inScheme rdf:resource="https://w3id.org/italia/controlled-vocabulary/classifications-for-public-services/life-business-event/life-event"/>
    <skos:definition xml:lang="en">This life event groups public services related to moving or changing address both for Italian citizens and foreigns who are in the country</skos:definition>
    <clvapit:hasRankOrder>1</clvapit:hasRankOrder>
    <skos:definition xml:lang="it">Questo evento della vita raggruppa servizi pubblici relativi al cambio di residenza o di domicilio sia per cittadini italiani sia per cittadini stranieri presenti nel territorio</skos:definition>
    <rdf:type rdf:resource="http://www.w3.org/2004/02/skos/core#Concept"/>
    <dct:identifier>9</dct:identifier>
  </rdf:Description>
  <rdf:Description rdf:about="http://dati.gov.it/data/resource/Distribution/LE_CSV">
    <rdf:type rdf:resource="http://dati.gov.it/onto/dcatapit#Distribution"/>
    <dct:title xml:lang="it">Distribuzione CSV eventi della vita</dct:title>
    <dct:description xml:lang="en">This is the distribution in CSV of the Linked Open Dataset of the controlled vocabulary related to the life events used in the Italian national catalogue of public services</dct:description>
    <dcat:downloadURL rdf:resource="https://raw.githubusercontent.com/italia/dati-semantic-assets/master/VocabolariControllati/classifications-for-public-services/life-busines-event/life-event/life-event.csv"/>
    <dct:title xml:lang="en">CSV distribution life events</dct:title>
    <dct:license rdf:resource="https://w3id.org/italia/controlled-vocabulary/licences/A21_CCBY40"/>
    <dct:description xml:lang="it">Questa è la distribuzione CSV del dataset Linked Open Data del vocabolario controllato sulla classificazione degli eventi della vita usati nel catalogo nazionale per i servizi pubblici</dct:description>
    <dct:format rdf:resource="http://publications.europa.eu/resource/authority/file-type/XLSX"/>
    <dcat:accessURL rdf:resource="https://raw.githubusercontent.com/italia/dati-semantic-assets/master/VocabolariControllati/classifications-for-public-services/life-busines-event/life-event"/>
  </rdf:Description>
  <rdf:Description rdf:about="https://w3id.org/italia/controlled-vocabulary/classifications-for-public-services/life-business-event/life-event">
    <dcat:theme rdf:resource="http://publications.europa.eu/resource/authority/data-theme/GOVE"/>
    <skos:hasTopConcept rdf:resource="https://w3id.org/italia/controlled-vocabulary/classifications-for-public-services/life-business-event/life-event/5"/>
    <dct:language rdf:resource="http://publications.europa.eu/resource/authority/language/DEU"/>
    <skos:hasTopConcept rdf:resource="https://w3id.org/italia/controlled-vocabulary/classifications-for-public-services/life-business-event/life-event/13"/>
    <skos:hasTopConcept rdf:resource="https://w3id.org/italia/controlled-vocabulary/classifications-for-public-services/life-business-event/life-event/7"/>
    <rdf:type rdf:resource="http://www.w3.org/ns/adms#Asset"/>
    <dct:issued rdf:datatype="http://www.w3.org/2001/XMLSchema#date">2017-10-20</dct:issued>
    <dct:description xml:lang="it">Vocabolario controllato della classificazione degli eventi della vita utilizzato nel catalogo nazionale dei servizi pubblici. Le traduzioni in tedesco sono state fornite da Ivo Planoetscher della Pronvicia Autonoma di Bolzano</dct:description>
    <skos:hasTopConcept rdf:resource="https://w3id.org/italia/controlled-vocabulary/classifications-for-public-services/life-business-event/life-event/16"/>
    <skos:hasTopConcept rdf:resource="https://w3id.org/italia/controlled-vocabulary/classifications-for-public-services/life-business-event/life-event/14"/>
    <skos:hasTopConcept rdf:resource="https://w3id.org/italia/controlled-vocabulary/classifications-for-public-services/life-business-event/life-event/2"/>
    <dct:modified rdf:datatype="http://www.w3.org/2001/XMLSchema#date">2018-03-14</dct:modified>
    <dct:description xml:lang="en">Controlled Vocabulary on the classification of the life events for the Italian catalogue of public services. The translations in German were provided by Ivo Planoetscher of the Autonomous Province of Bolzano</dct:description>
    <dcat:keyword xml:lang="it">evento della vita</dcat:keyword>
    <skos:hasTopConcept rdf:resource="https://w3id.org/italia/controlled-vocabulary/classifications-for-public-services/life-business-event/life-event/6"/>
    <dct:subject rdf:resource="http://eurovoc.europa.eu/246146"/>
    <dct:rightsHolder rdf:resource="http://spcdata.digitpa.gov.it/browse/page/Amministrazione/agid"/>
    <dcat:keyword xml:lang="it">evento</dcat:keyword>
    <skos:hasTopConcept rdf:resource="https://w3id.org/italia/controlled-vocabulary/classifications-for-public-services/life-business-event/life-event/12"/>
    <skos:hasTopConcept rdf:resource="https://w3id.org/italia/controlled-vocabulary/classifications-for-public-services/life-business-event/life-event/9"/>
    <skos:hasTopConcept rdf:resource="https://w3id.org/italia/controlled-vocabulary/classifications-for-public-services/life-business-event/life-event/15"/>
    <dcat:keyword xml:lang="en">life event</dcat:keyword>
    <skos:hasTopConcept rdf:resource="https://w3id.org/italia/controlled-vocabulary/classifications-for-public-services/life-business-event/life-event/4"/>
    <dcat:distribution rdf:resource="http://dati.gov.it/data/resource/Distribution/LE_CSV"/>
    <skos:hasTopConcept rdf:resource="https://w3id.org/italia/controlled-vocabulary/classifications-for-public-services/life-business-event/life-event/8"/>
    <dcat:keyword xml:lang="en">public service</dcat:keyword>
    <skos:hasTopConcept rdf:resource="https://w3id.org/italia/controlled-vocabulary/classifications-for-public-services/life-business-event/life-event/3"/>
    <dct:conformsTo rdf:resource="http://dati.gov.it/data/resource/Standard/SKOS"/>
    <dct:title xml:lang="it">Eventi della Vita</dct:title>
    <dct:identifier>agid:D.8</dct:identifier>
    <skos:hasTopConcept rdf:resource="https://w3id.org/italia/controlled-vocabulary/classifications-for-public-services/life-business-event/life-event/10"/>
    <dct:accrualPeriodicity rdf:resource="http://publications.europa.eu/resource/authority/frequency/IRREG"/>
    <rdfs:label xml:lang="en">Life Events</rdfs:label>
    <dct:publisher rdf:resource="http://spcdata.digitpa.gov.it/browse/page/Amministrazione/agid"/>
    <dcat:keyword xml:lang="it">servizio pubblico</dcat:keyword>
    <rdf:type rdf:resource="http://dati.gov.it/onto/dcatapit#Dataset"/>
    <dct:subject rdf:resource="http://eurovoc.europa.eu/246051"/>
    <rdfs:isDefinedBy rdf:resource="https://w3id.org/italia/controlled-vocabulary/classifications-for-public-services/life-business-event/life-event"/>
    <skos:hasTopConcept rdf:resource="https://w3id.org/italia/controlled-vocabulary/classifications-for-public-services/life-business-event/life-event/17"/>
    <dcat:distribution rdf:resource="http://dati.gov.it/data/resource/Distribution/LE_RDF_XML"/>
    <owl:versionInfo>0.1</owl:versionInfo>
    <dct:subject rdf:resource="http://eurovoc.europa.eu/100169"/>
    <xkos:numberOfLevels>1</xkos:numberOfLevels>
    <dct:creator rdf:resource="http://spcdata.digitpa.gov.it/browse/page/Amministrazione/agid"/>
    <dcat:distribution rdf:resource="http://dati.gov.it/data/resource/Distribution/LE_JSON_LD"/>
    <adms:representationTechnique rdf:resource="http://purl.org/adms/representationtechnique/SKOS"/>
    <dcat:contactPoint rdf:resource="http://dati.gov.it/data/resource/ContactPoint/voc_AgID"/>
    <dct:language rdf:resource="http://publications.europa.eu/resource/authority/language/ENG"/>
    <rdfs:comment xml:lang="en">Classification of the life events for the Italian catalogue of public services</rdfs:comment>
    <dct:title xml:lang="en">Life Events</dct:title>
    <dcat:distribution rdf:resource="http://dati.gov.it/data/resource/Distribution/LE_RDF_Turtle"/>
    <skos:hasTopConcept rdf:resource="https://w3id.org/italia/controlled-vocabulary/classifications-for-public-services/life-business-event/life-event/1"/>
    <rdf:type rdf:resource="http://www.w3.org/2004/02/skos/core#ConceptScheme"/>
    <rdfs:label xml:lang="it">Eventi della Vita</rdfs:label>
    <dcat:keyword xml:lang="en">event</dcat:keyword>
    <skos:hasTopConcept rdf:resource="https://w3id.org/italia/controlled-vocabulary/classifications-for-public-services/life-business-event/life-event/19"/>
    <rdfs:comment xml:lang="it">Classificazione degli eventi della vita per il catalogo italiano dei servizi pubblici</rdfs:comment>
    <dct:language rdf:resource="http://publications.europa.eu/resource/authority/language/ITA"/>
    <dct:type rdf:resource="http://purl.org/adms/assettype/CodeList"/>
    <dcat:distribution rdf:resource="http://dati.gov.it/data/resource/Distribution/LE_XLSX"/>
    <skos:hasTopConcept rdf:resource="https://w3id.org/italia/controlled-vocabulary/classifications-for-public-services/life-business-event/life-event/11"/>
    <skos:hasTopConcept rdf:resource="https://w3id.org/italia/controlled-vocabulary/classifications-for-public-services/life-business-event/life-event/18"/>
  </rdf:Description>
  <rdf:Description rdf:about="https://w3id.org/italia/controlled-vocabulary/classifications-for-public-services/life-business-event/life-event/13">
    <clvapit:hasRankOrder>1</clvapit:hasRankOrder>
    <skos:prefLabel xml:lang="en">Marrying and/or changing martal status</skos:prefLabel>
    <skos:definition xml:lang="it">Questo evento della vita raggruppa servizi pubblici relativi a una relazione ufficiale di una persona, come per esempio il matrimonio, l'unione civile, il divorzio,...</skos:definition>
    <skos:notation>13</skos:notation>
    <skos:prefLabel xml:lang="de">Heirat und/oder Änderung des Familienstandes</skos:prefLabel>
    <rdf:type rdf:resource="https://w3id.org/italia/onto/CPSV/LifeEvent"/>
    <skos:inScheme rdf:resource="https://w3id.org/italia/controlled-vocabulary/classifications-for-public-services/life-business-event/life-event"/>
    <skos:definition xml:lang="en">This life event groups public services related to a person’s official relationship, for instance marriage, registered partnership, divorce…</skos:definition>
    <dct:identifier>13</dct:identifier>
    <skos:prefLabel xml:lang="it">Matrimonio e/o cambio stato civile</skos:prefLabel>
    <rdf:type rdf:resource="http://www.w3.org/2004/02/skos/core#Concept"/>
  </rdf:Description>
  <rdf:Description rdf:about="https://w3id.org/italia/controlled-vocabulary/classifications-for-public-services/life-business-event/life-event/16">
    <skos:prefLabel xml:lang="en">Reporting a crime (smaller offences, e.g., theft, burglary, etc)</skos:prefLabel>
    <dct:identifier>16</dct:identifier>
    <skos:notation>16</skos:notation>
    <rdf:type rdf:resource="http://www.w3.org/2004/02/skos/core#Concept"/>
    <rdf:type rdf:resource="https://w3id.org/italia/onto/CPSV/LifeEvent"/>
    <skos:prefLabel xml:lang="de">Meldung einer Straftat (kleinere Straftaten, z.B. Diebstahl, Einbruchdiebstahl, usw.)</skos:prefLabel>
    <skos:definition xml:lang="en">This life event groups public services related to a crime, for instance in case you are the committer of that crime, or the victim or witness of a particular crime.</skos:definition>
    <skos:inScheme rdf:resource="https://w3id.org/italia/controlled-vocabulary/classifications-for-public-services/life-business-event/life-event"/>
    <skos:definition xml:lang="it">Questo evento della vita raggruppa servizi pubblici relativi a un crimine, per esempio nel caso in cui una persona è vittima o testimone di uno specifico crimine, ecc.</skos:definition>
    <clvapit:hasRankOrder>1</clvapit:hasRankOrder>
    <skos:prefLabel xml:lang="it">Denuncia crimini</skos:prefLabel>
  </rdf:Description>
  <rdf:Description rdf:about="http://www.w3.org/ns/adms#representationTechnique">
    <rdf:type rdf:resource="http://www.w3.org/2000/01/rdf-schema#Property"/>
  </rdf:Description>
  <rdf:Description rdf:about="https://w3id.org/italia/controlled-vocabulary/classifications-for-public-services/life-business-event/life-event/6">
    <skos:prefLabel xml:lang="en">Registering/owning a vehicle</skos:prefLabel>
    <skos:notation>6</skos:notation>
    <rdf:type rdf:resource="https://w3id.org/italia/onto/CPSV/LifeEvent"/>
    <skos:prefLabel xml:lang="it">Registrazione/possesso veicolo</skos:prefLabel>
    <skos:prefLabel xml:lang="de">Fahrzeugregistrierung/-besitz</skos:prefLabel>
    <clvapit:hasRankOrder>1</clvapit:hasRankOrder>
    <skos:inScheme rdf:resource="https://w3id.org/italia/controlled-vocabulary/classifications-for-public-services/life-business-event/life-event"/>
    <dct:identifier>6</dct:identifier>
    <rdf:type rdf:resource="http://www.w3.org/2004/02/skos/core#Concept"/>
    <skos:definition xml:lang="en">This life event groups public services related to the registration or the ownership of a vehicle such as a car, a motorcycle, etc.</skos:definition>
    <skos:definition xml:lang="it">Questo evento della vita raggruppo servizi pubblici relativi alla registrazione e al possesso di un veicolo come una macchina, una moto, ecc.</skos:definition>
  </rdf:Description>
  <rdf:Description rdf:about="https://w3id.org/italia/controlled-vocabulary/classifications-for-public-services/life-business-event/life-event/7">
    <rdf:type rdf:resource="https://w3id.org/italia/onto/CPSV/LifeEvent"/>
    <skos:notation>7</skos:notation>
    <skos:definition xml:lang="it">Questo evento della vita raggruppa servizi pubblici relativi all'accesso al trasporto pubblico come per esempio il rinnovo di un abbonamento, l'acquisto di un biglietto singolo per l'autobus, ecc. </skos:definition>
    <clvapit:hasRankOrder>1</clvapit:hasRankOrder>
    <dct:identifier>7</dct:identifier>
    <skos:prefLabel xml:lang="it">Accesso al trasporto pubblico</skos:prefLabel>
    <skos:definition xml:lang="en">This life event groups public services related to the access to the public transportation such as for instance the renewal of a subscription, the purchase of a single bus ticket, etc.</skos:definition>
    <skos:inScheme rdf:resource="https://w3id.org/italia/controlled-vocabulary/classifications-for-public-services/life-business-event/life-event"/>
    <rdf:type rdf:resource="http://www.w3.org/2004/02/skos/core#Concept"/>
    <skos:prefLabel xml:lang="de">Zugang zu öffentlichen Verkehrsmitteln</skos:prefLabel>
    <skos:prefLabel xml:lang="en">Access to public transportation</skos:prefLabel>
  </rdf:Description>
  <rdf:Description rdf:about="http://dati.gov.it/data/resource/Distribution/LE_RDF_Turtle">
    <dct:description xml:lang="it">Questa è la distribuzione RDF/Turtle del dataset Linked Open Data del vocabolario controllato sulla classificazione degli eventi della vita usati nel catalogo nazionale per i servizi pubblici</dct:description>
    <dct:title xml:lang="en">RDF/Turtle distribution life events</dct:title>
    <dct:format rdf:resource="http://publications.europa.eu/resource/authority/file-type/RDF_TURTLE"/>
    <dct:license rdf:resource="https://w3id.org/italia/controlled-vocabulary/licences/A21_CCBY40"/>
    <rdf:type rdf:resource="http://dati.gov.it/onto/dcatapit#Distribution"/>
    <dcat:downloadURL rdf:resource="https://raw.githubusercontent.com/italia/dati-semantic-assets/master/VocabolariControllati/classifications-for-public-services/life-busines-event/life-event/life-event.ttl"/>
    <dcat:accessURL rdf:resource="https://raw.githubusercontent.com/italia/dati-semantic-assets/master/VocabolariControllati/classifications-for-public-services/life-busines-event/life-event"/>
    <dct:description xml:lang="en">This is the distribution in RDF/Turtle of the Linked Open Dataset of the controlled vocabulary related to the life events used in the Italian national catalogue of public services</dct:description>
    <dct:title xml:lang="it">Distribuzione RDF/Turtle eventi della vita</dct:title>
  </rdf:Description>
  <rdf:Description rdf:about="https://w3id.org/italia/controlled-vocabulary/classifications-for-public-services/life-business-event/life-event/3">
    <skos:notation>3</skos:notation>
    <skos:prefLabel xml:lang="en">Looking for a job, starting a new job, becoming unemployed</skos:prefLabel>
    <skos:inScheme rdf:resource="https://w3id.org/italia/controlled-vocabulary/classifications-for-public-services/life-business-event/life-event"/>
    <dct:identifier>3</dct:identifier>
    <skos:definition xml:lang="en">This life event groups public services for when someone looks for a new job, starts a new job, leaves or quits a particular job on his own, or when someone loses his job </skos:definition>
    <rdf:type rdf:resource="http://www.w3.org/2004/02/skos/core#Concept"/>
    <skos:prefLabel xml:lang="de">Arbeit suchen, einen neuen Job beginnen, arbeitslos werden</skos:prefLabel>
    <skos:prefLabel xml:lang="it">Ricerca di lavoro, avvio nuovo lavoro, disoccupazione</skos:prefLabel>
    <rdf:type rdf:resource="https://w3id.org/italia/onto/CPSV/LifeEvent"/>
    <skos:definition xml:lang="it">Questo evento della vita raggruppa servizi pubblici utili a quelli che cercano un nuovo lavoro, iniziano un nuovo lavoro, lasciano un lavoro spontaneamente o perdono il lavoro</skos:definition>
    <clvapit:hasRankOrder>1</clvapit:hasRankOrder>
  </rdf:Description>
  <rdf:Description rdf:about="https://w3id.org/italia/controlled-vocabulary/classifications-for-public-services/life-business-event/life-event/15">
    <skos:notation>15</skos:notation>
    <skos:prefLabel xml:lang="de">Einen Arzttermin vereinbaren / absagen</skos:prefLabel>
    <dct:identifier>15</dct:identifier>
    <skos:prefLabel xml:lang="en">Making/cancelling a doctor's appointment</skos:prefLabel>
    <clvapit:hasRankOrder>1</clvapit:hasRankOrder>
    <skos:inScheme rdf:resource="https://w3id.org/italia/controlled-vocabulary/classifications-for-public-services/life-business-event/life-event"/>
    <skos:prefLabel xml:lang="it">Prenotazione e disdetta visite/esami</skos:prefLabel>
    <rdf:type rdf:resource="http://www.w3.org/2004/02/skos/core#Concept"/>
    <rdf:type rdf:resource="https://w3id.org/italia/onto/CPSV/LifeEvent"/>
  </rdf:Description>
  <rdf:Description rdf:about="http://dati.gov.it/data/resource/Standard/SKOS">
    <rdf:type rdf:resource="http://dati.gov.it/onto/dcatapit#Standard"/>
    <rdf:type rdf:resource="http://purl.org/dc/terms/Standard"/>
    <dct:identifier>SKOS</dct:identifier>
    <dct:title>Simple Knowledge Organization System - SKOS</dct:title>
    <dct:description>The Simple Knowledge Organization System (SKOS) is a common data model for sharing and linking knowledge organization systems via the Web</dct:description>
  </rdf:Description>
  <rdf:Description rdf:about="https://w3id.org/italia/controlled-vocabulary/classifications-for-public-services/life-business-event/life-event/19">
    <skos:prefLabel xml:lang="it">Possesso, cura, smarrimento animale da compagnia</skos:prefLabel>
    <rdf:type rdf:resource="https://w3id.org/italia/onto/CPSV/LifeEvent"/>
    <skos:notation>19</skos:notation>
    <rdf:type rdf:resource="http://www.w3.org/2004/02/skos/core#Concept"/>
    <skos:prefLabel xml:lang="en">Owning, taking care, losing pets</skos:prefLabel>
    <skos:definition xml:lang="en">This life groups public services related to the people who owns a pet. Examples include: communicate the transfer of a dog to another, the death of a dog, etc.</skos:definition>
    <skos:inScheme rdf:resource="https://w3id.org/italia/controlled-vocabulary/classifications-for-public-services/life-business-event/life-event"/>
    <clvapit:hasRankOrder>1</clvapit:hasRankOrder>
    <skos:prefLabel xml:lang="de">Besitz, Pflege, Verlust von Haustieren</skos:prefLabel>
    <skos:definition xml:lang="it">Questo evento della vita raggruppa servizi pubbici che possono essere utilizzati dalle persone che hanno un animale da compagnia. Esempi includono: comunicazione di cessione di un cane ad un altro, decesso di un cane, ecc.</skos:definition>
    <dct:identifier>19</dct:identifier>
  </rdf:Description>
  <rdf:Description rdf:about="http://xmlns.com/foaf/0.1/Agent">
    <rdf:type rdf:resource="http://www.w3.org/2000/01/rdf-schema#Class"/>
  </rdf:Description>
  <rdf:Description rdf:about="http://dati.gov.it/data/resource/Distribution/LE_XLSX">
    <dct:title xml:lang="en">XLSX distribution life events</dct:title>
    <dcat:accessURL rdf:resource="https://raw.githubusercontent.com/italia/dati-semantic-assets/master/VocabolariControllati/classifications-for-public-services/life-busines-event/life-event"/>
    <dct:license rdf:resource="https://w3id.org/italia/controlled-vocabulary/licences/A21_CCBY40"/>
    <dct:description xml:lang="en">This is the distribution in XLSX of the Linked Open Dataset of the controlled vocabulary related to the life events used in the Italian national catalogue of public services</dct:description>
    <dct:description xml:lang="it">Questa è la distribuzione XLSX del dataset Linked Open Data del vocabolario controllato sulla classificazione degli eventi della vita usati nel catalogo nazionale per i servizi pubblici</dct:description>
    <dct:title xml:lang="it">Distribuzione XLSX eventi della vita</dct:title>
    <dct:format rdf:resource="http://publications.europa.eu/resource/authority/file-type/XLSX"/>
    <dcat:downloadURL rdf:resource="https://raw.githubusercontent.com/italia/dati-semantic-assets/master/VocabolariControllati/classifications-for-public-services/life-busines-event/life-event/life-event.xlsx"/>
    <rdf:type rdf:resource="http://dati.gov.it/onto/dcatapit#Distribution"/>
  </rdf:Description>
  <rdf:Description rdf:about="https://w3id.org/italia/controlled-vocabulary/classifications-for-public-services/life-business-event/life-event/5">
    <skos:inScheme rdf:resource="https://w3id.org/italia/controlled-vocabulary/classifications-for-public-services/life-business-event/life-event"/>
    <skos:definition xml:lang="it">Questo evento della vita raggruppa servizi pubblici relativi alla guida di un veicolo per esempio una macchina, una moto</skos:definition>
    <dct:identifier>5</dct:identifier>
    <skos:prefLabel xml:lang="en">Applying to a driver's licence (or renewing an existing one)</skos:prefLabel>
    <rdf:type rdf:resource="https://w3id.org/italia/onto/CPSV/LifeEvent"/>
    <skos:prefLabel xml:lang="it">Richiesta o rinnovo patente</skos:prefLabel>
    <rdf:type rdf:resource="http://www.w3.org/2004/02/skos/core#Concept"/>
    <skos:notation>5</skos:notation>
    <clvapit:hasRankOrder>1</clvapit:hasRankOrder>
    <skos:definition xml:lang="en">This life event groups public services related to driving a vehicle, for instance car, motorcycle.</skos:definition>
    <skos:prefLabel xml:lang="de">Beantragung eines Führerscheins (oder Erneuerung eines bestehenden Führerscheins)</skos:prefLabel>
  </rdf:Description>
  <rdf:Description rdf:about="https://w3id.org/italia/controlled-vocabulary/classifications-for-public-services/life-business-event/life-event/4">
    <rdf:type rdf:resource="http://www.w3.org/2004/02/skos/core#Concept"/>
    <skos:definition xml:lang="en">This life event groups public services related to when someone retires from his job or becomes a senior.</skos:definition>
    <clvapit:hasRankOrder>1</clvapit:hasRankOrder>
    <skos:notation>4</skos:notation>
    <skos:inScheme rdf:resource="https://w3id.org/italia/controlled-vocabulary/classifications-for-public-services/life-business-event/life-event"/>
    <dct:identifier>4</dct:identifier>
    <skos:definition xml:lang="it">Questo evento della vita raggruppa servizi pubblici relativi al pensionamento di una persona</skos:definition>
    <skos:prefLabel xml:lang="de">Pensionierung</skos:prefLabel>
    <skos:prefLabel xml:lang="it">Pensionamento</skos:prefLabel>
    <rdf:type rdf:resource="https://w3id.org/italia/onto/CPSV/LifeEvent"/>
    <skos:prefLabel xml:lang="en">Retirement</skos:prefLabel>
  </rdf:Description>
  <rdf:Description rdf:about="http://purl.org/dc/terms/accrualPeriodicity">
    <rdf:type rdf:resource="http://www.w3.org/2000/01/rdf-schema#Property"/>
  </rdf:Description>
  <rdf:Description rdf:about="http://www.w3.org/2004/02/skos/core#Concept">
    <rdf:type rdf:resource="http://www.w3.org/2000/01/rdf-schema#Class"/>
  </rdf:Description>
  <rdf:Description rdf:about="https://w3id.org/italia/controlled-vocabulary/classifications-for-public-services/life-business-event/life-event/12">
    <rdf:type rdf:resource="https://w3id.org/italia/onto/CPSV/LifeEvent"/>
    <skos:notation>12</skos:notation>
    <skos:definition xml:lang="en">This life event groups public services related to becoming a caretaker for a child, for instance in case of giving birth, adopting, receiving a foster child…</skos:definition>
    <clvapit:hasRankOrder>1</clvapit:hasRankOrder>
    <dct:identifier>12</dct:identifier>
    <skos:prefLabel xml:lang="de">Die Geburt eines Kindes erklären und / oder einen Geburtszuschuss beantragen</skos:prefLabel>
    <skos:prefLabel xml:lang="en">Declaring the birth of a child and/or applying for a birth grand</skos:prefLabel>
    <skos:inScheme rdf:resource="https://w3id.org/italia/controlled-vocabulary/classifications-for-public-services/life-business-event/life-event"/>
    <rdf:type rdf:resource="http://www.w3.org/2004/02/skos/core#Concept"/>
    <skos:prefLabel xml:lang="it">Nascita di un bambino, richiesta adozioni</skos:prefLabel>
    <skos:definition xml:lang="it">Questo evento della vita raggruppa servizi pubblici relativi alla nascita di un bambino, all'adozione di un bambino, ecc.</skos:definition>
  </rdf:Description>
  <rdf:Description rdf:about="https://w3id.org/italia/controlled-vocabulary/classifications-for-public-services/life-business-event/life-event/14">
    <skos:inScheme rdf:resource="https://w3id.org/italia/controlled-vocabulary/classifications-for-public-services/life-business-event/life-event"/>
    <skos:prefLabel xml:lang="it">Morte ed eredità</skos:prefLabel>
    <skos:notation>14</skos:notation>
    <rdf:type rdf:resource="http://www.w3.org/2004/02/skos/core#Concept"/>
    <dct:identifier>14</dct:identifier>
    <skos:prefLabel xml:lang="en">Death of a close relative and/or starting an inheritance procedure</skos:prefLabel>
    <rdf:type rdf:resource="https://w3id.org/italia/onto/CPSV/LifeEvent"/>
    <skos:definition xml:lang="it">Questo evento della vita raggruppa servizi pubblici necessari quando una persona muore (per esempio notifica alle autorità, gestione del funerale, ecc.) e quelli relativi all'eredità e alle donazioni</skos:definition>
    <skos:prefLabel xml:lang="de">Tod eines nahen Verwandten und/oder Einleitung eines Erbschaftsverfahrens</skos:prefLabel>
    <skos:definition xml:lang="en">This life event groups public services that relate to when a relative passes a way, and cover the public services directly related to the decease of that person (for instance notifying the authorities, arranging the funeral…), as well as related to settling inheritance and donations.</skos:definition>
    <clvapit:hasRankOrder>1</clvapit:hasRankOrder>
  </rdf:Description>
  <rdf:Description rdf:about="http://dati.gov.it/data/resource/Distribution/LE_JSON_LD">
    <dct:license rdf:resource="https://w3id.org/italia/controlled-vocabulary/licences/A21_CCBY40"/>
    <rdf:type rdf:resource="http://dati.gov.it/onto/dcatapit#Distribution"/>
    <dct:title xml:lang="it">Distribuzione JSON_LD eventi della vita</dct:title>
    <dct:description xml:lang="it">Questa è la distribuzione JSON_LD del dataset Linked Open Data del vocabolario controllato sulla classificazione degli eventi della vita usati nel catalogo nazionale per i servizi pubblici</dct:description>
    <dct:description xml:lang="en">This is the distribution in JSON_LD of the Linked Open Dataset of the controlled vocabulary related to the life events used in the Italian national catalogue of public services</dct:description>
    <dcat:downloadURL rdf:resource="https://raw.githubusercontent.com/italia/dati-semantic-assets/master/VocabolariControllati/classifications-for-public-services/life-busines-event/life-event/life-event.jsonld"/>
    <dct:format rdf:resource="http://publications.europa.eu/resource/authority/file-type/JSON_LD"/>
    <dct:title xml:lang="en">JSON_LD distribution life events</dct:title>
    <dcat:accessURL rdf:resource="https://raw.githubusercontent.com/italia/dati-semantic-assets/master/VocabolariControllati/classifications-for-public-services/life-busines-event/life-event"/>
  </rdf:Description>
  <rdf:Description rdf:about="http://dati.gov.it/onto/dcatapit#Standard">
    <rdf:type rdf:resource="http://www.w3.org/2000/01/rdf-schema#Class"/>
  </rdf:Description>
  <rdf:Description rdf:about="http://www.w3.org/2006/vcard/ns#fn">
    <rdf:type rdf:resource="http://www.w3.org/2000/01/rdf-schema#Property"/>
  </rdf:Description>
  <rdf:Description rdf:about="http://purl.org/dc/terms/language">
    <rdf:type rdf:resource="http://www.w3.org/2000/01/rdf-schema#Property"/>
  </rdf:Description>
  <rdf:Description rdf:about="http://spcdata.digitpa.gov.it/browse/page/Amministrazione/agid">
    <foaf:name xml:lang="it">Agenzia per l'Italia Digitale</foaf:name>
    <foaf:name xml:lang="en">Italian Digital Agency</foaf:name>
    <rdf:type rdf:resource="http://dati.gov.it/onto/dcatapit#Agent"/>
    <dct:identifier>agid</dct:identifier>
    <rdf:type rdf:resource="http://xmlns.com/foaf/0.1/Agent"/>
  </rdf:Description>
  <rdf:Description rdf:about="http://purl.org/dc/terms/issued">
    <rdf:type rdf:resource="http://www.w3.org/2000/01/rdf-schema#Property"/>
  </rdf:Description>
  <rdf:Description rdf:about="https://w3id.org/italia/controlled-vocabulary/classifications-for-public-services/life-business-event/life-event/11">
    <dct:identifier>11</dct:identifier>
    <rdf:type rdf:resource="https://w3id.org/italia/onto/CPSV/LifeEvent"/>
    <rdf:type rdf:resource="http://www.w3.org/2004/02/skos/core#Concept"/>
    <skos:notation>11</skos:notation>
    <skos:prefLabel xml:lang="de">Benötigung eines Reisepasses / Visums oder Unterstützung bei der Reise in ein anderes Land</skos:prefLabel>
    <clvapit:hasRankOrder>1</clvapit:hasRankOrder>
    <skos:definition xml:lang="en">This life events groups public services related to what you need to do when travelling abroad, for instance getting an international passport or driving license, getting a visa, getting vaccination…</skos:definition>
    <skos:definition xml:lang="it">Questo evento della vita raggruppa servizi pubblici relativi alle necessità di una persona nel caso di viaggi all'estero. Per esempio: ottenere un passaporto, un visto, una vaccinazione, ecc.</skos:definition>
    <skos:inScheme rdf:resource="https://w3id.org/italia/controlled-vocabulary/classifications-for-public-services/life-business-event/life-event"/>
    <skos:prefLabel xml:lang="it">Richiesta passaporto, visto e assistenza viaggi internazionali</skos:prefLabel>
    <skos:prefLabel xml:lang="en">Needing a passport/visa or assistance to travel to another country</skos:prefLabel>
  </rdf:Description>
  <rdf:Description rdf:about="http://purl.org/dc/terms/format">
    <rdf:type rdf:resource="http://www.w3.org/2000/01/rdf-schema#Property"/>
  </rdf:Description>
  <rdf:Description rdf:about="http://dati.gov.it/onto/dcatapit#Agent">
    <rdf:type rdf:resource="http://www.w3.org/2000/01/rdf-schema#Class"/>
  </rdf:Description>
  <rdf:Description rdf:about="http://purl.org/dc/terms/conformsTo">
    <rdf:type rdf:resource="http://www.w3.org/2000/01/rdf-schema#Property"/>
  </rdf:Description>
  <rdf:Description rdf:about="https://w3id.org/italia/controlled-vocabulary/classifications-for-public-services/life-business-event/life-event/8">
    <skos:definition xml:lang="it">Questo evento della vita raggruppa servizi pubblici relativi a un posto dove una persona vive: Esempi di servizi pubblici includono: comprare una casa o una parte di terreno, costruire o ristrutturare un appartamento/casa, ecc.</skos:definition>
    <skos:definition xml:lang="en">This life event groups public services related to a person’s place of living, for instance, buying a house or a piece of land, building, renting a house or apartment…</skos:definition>
    <rdf:type rdf:resource="https://w3id.org/italia/onto/CPSV/LifeEvent"/>
    <rdf:type rdf:resource="http://www.w3.org/2004/02/skos/core#Concept"/>
    <skos:prefLabel xml:lang="it">Compravendita/affitto casa/edifici/terreni, costruzione o ristrutturazione casa/edificio</skos:prefLabel>
    <skos:inScheme rdf:resource="https://w3id.org/italia/controlled-vocabulary/classifications-for-public-services/life-business-event/life-event"/>
    <skos:prefLabel xml:lang="de">Kaufen/Mieten eines Hauses/Gebäudes/Grundstücks, Bauen, Renovieren eines Hauses/Gebäudes</skos:prefLabel>
    <skos:notation>8</skos:notation>
    <clvapit:hasRankOrder>1</clvapit:hasRankOrder>
    <dct:identifier>8</dct:identifier>
    <skos:prefLabel xml:lang="en">Buying/renting a house/building/land, building, renovating a house/building</skos:prefLabel>
  </rdf:Description>
  <rdf:Description rdf:about="https://w3id.org/italia/controlled-vocabulary/classifications-for-public-services/life-business-event/life-event/1">
    <rdf:type rdf:resource="http://www.w3.org/2004/02/skos/core#Concept"/>
    <rdf:type rdf:resource="https://w3id.org/italia/onto/CPSV/LifeEvent"/>
    <skos:prefLabel xml:lang="de">Einschreibung in die Schule/Universität und/oder Bewerbung um ein Studienstipendium</skos:prefLabel>
    <skos:notation>1</skos:notation>
    <skos:inScheme rdf:resource="https://w3id.org/italia/controlled-vocabulary/classifications-for-public-services/life-business-event/life-event"/>
    <skos:definition xml:lang="it">Questo evento della vita raggruppa qualsiasi servizio pubblico relativo all'educazione, per esempio l'educazione pre-scolastica, la scuola elementare, la scuola media e la scuola superiore, l'università, la borsa di studio, ...</skos:definition>
    <clvapit:hasRankOrder>1</clvapit:hasRankOrder>
    <skos:definition xml:lang="en">This life event groups any public service related to education, for example pre-school education, elementary school, higher education and university, a study grant, ...</skos:definition>
    <skos:prefLabel xml:lang="en">Enrolling in school/university and/or applying for a study grant</skos:prefLabel>
    <skos:prefLabel xml:lang="it">Iscrizione Scuola/Università e/o richiesta borsa di studio</skos:prefLabel>
    <dct:identifier>1</dct:identifier>
  </rdf:Description>
  <rdf:Description rdf:about="http://dati.gov.it/onto/dcatapit#Organization">
    <rdf:type rdf:resource="http://www.w3.org/2000/01/rdf-schema#Class"/>
  </rdf:Description>
  <rdf:Description rdf:about="https://w3id.org/italia/controlled-vocabulary/classifications-for-public-services/life-business-event/life-event/17">
    <rdf:type rdf:resource="https://w3id.org/italia/onto/CPSV/LifeEvent"/>
    <clvapit:hasRankOrder>1</clvapit:hasRankOrder>
    <skos:inScheme rdf:resource="https://w3id.org/italia/controlled-vocabulary/classifications-for-public-services/life-business-event/life-event"/>
    <rdf:type rdf:resource="http://www.w3.org/2004/02/skos/core#Concept"/>
    <skos:notation>17</skos:notation>
    <skos:prefLabel xml:lang="de">Einkommenssteuer erklären, Beiträge bezahlen</skos:prefLabel>
    <dct:identifier>17</dct:identifier>
    <skos:prefLabel xml:lang="it">Dichiarazione dei redditi, versamento e riscossione tributi/imposte e contributi</skos:prefLabel>
    <skos:prefLabel xml:lang="en">Declaring income taxes, paying contributions</skos:prefLabel>
  </rdf:Description>
  <rdf:Description rdf:about="http://dati.gov.it/data/resource/ContactPoint/voc_AgID">
    <vcard:fn>banche dati e open data</vcard:fn>
    <rdf:type rdf:resource="http://www.w3.org/2006/vcard/ns#Kind"/>
    <rdf:type rdf:resource="http://dati.gov.it/onto/dcatapit#Organization"/>
    <rdf:type rdf:resource="http://www.w3.org/2006/vcard/ns#Organization"/>
    <vcard:hasEmail rdf:resource="mailto:info@dati.gov.it"/>
  </rdf:Description>
  <rdf:Description rdf:about="http://dati.gov.it/onto/dcatapit#Distribution">
    <rdf:type rdf:resource="http://www.w3.org/2000/01/rdf-schema#Class"/>
  </rdf:Description>
  <rdf:Description rdf:about="http://www.w3.org/ns/dcat#accessURL">
    <rdf:type rdf:resource="http://www.w3.org/2000/01/rdf-schema#Property"/>
  </rdf:Description>
  <rdf:Description rdf:about="http://purl.org/dc/terms/publisher">
    <rdf:type rdf:resource="http://www.w3.org/2000/01/rdf-schema#Property"/>
  </rdf:Description>
  <rdf:Description rdf:about="http://purl.org/dc/terms/rightsHolder">
    <rdf:type rdf:resource="http://www.w3.org/2000/01/rdf-schema#Property"/>
  </rdf:Description>
  <rdf:Description rdf:about="http://www.w3.org/2004/02/skos/core#prefLabel">
    <rdf:type rdf:resource="http://www.w3.org/2000/01/rdf-schema#Property"/>
  </rdf:Description>
  <rdf:Description rdf:about="http://www.w3.org/ns/dcat#contactPoint">
    <rdf:type rdf:resource="http://www.w3.org/2000/01/rdf-schema#Property"/>
  </rdf:Description>
  <rdf:Description rdf:about="http://purl.org/dc/terms/creator">
    <rdf:type rdf:resource="http://www.w3.org/2000/01/rdf-schema#Property"/>
  </rdf:Description>
  <rdf:Description rdf:about="http://purl.org/dc/terms/license">
    <rdf:type rdf:resource="http://www.w3.org/2000/01/rdf-schema#Property"/>
  </rdf:Description>
  <rdf:Description rdf:about="http://www.w3.org/2004/02/skos/core#ConceptScheme">
    <rdf:type rdf:resource="http://www.w3.org/2000/01/rdf-schema#Class"/>
  </rdf:Description>
  <rdf:Description rdf:about="http://rdf-vocabulary.ddialliance.org/xkos#numberOfLevels">
    <rdf:type rdf:resource="http://www.w3.org/2000/01/rdf-schema#Property"/>
  </rdf:Description>
  <rdf:Description rdf:about="http://purl.org/dc/terms/type">
    <rdf:type rdf:resource="http://www.w3.org/2000/01/rdf-schema#Property"/>
  </rdf:Description>
  <rdf:Description rdf:about="http://www.w3.org/2002/07/owl#versionInfo">
    <rdf:type rdf:resource="http://www.w3.org/2000/01/rdf-schema#Property"/>
  </rdf:Description>
  <rdf:Description rdf:about="http://purl.org/dc/terms/modified">
    <rdf:type rdf:resource="http://www.w3.org/2000/01/rdf-schema#Property"/>
  </rdf:Description>
  <rdf:Description rdf:about="http://www.w3.org/2004/02/skos/core#notation">
    <rdf:type rdf:resource="http://www.w3.org/2000/01/rdf-schema#Property"/>
  </rdf:Description>
  <rdf:Description rdf:about="http://purl.org/dc/terms/description">
    <rdf:type rdf:resource="http://www.w3.org/2000/01/rdf-schema#Property"/>
  </rdf:Description>
  <rdf:Description rdf:about="http://purl.org/dc/terms/Standard">
    <rdf:type rdf:resource="http://www.w3.org/2000/01/rdf-schema#Class"/>
  </rdf:Description>
  <rdf:Description rdf:about="http://xmlns.com/foaf/0.1/name">
    <rdf:type rdf:resource="http://www.w3.org/2000/01/rdf-schema#Property"/>
  </rdf:Description>
  <rdf:Description rdf:about="http://purl.org/dc/terms/subject">
    <rdf:type rdf:resource="http://www.w3.org/2000/01/rdf-schema#Property"/>
  </rdf:Description>
  <rdf:Description rdf:about="http://purl.org/dc/terms/title">
    <rdf:type rdf:resource="http://www.w3.org/2000/01/rdf-schema#Property"/>
  </rdf:Description>
  <rdf:Description rdf:about="http://purl.org/dc/terms/identifier">
    <rdf:type rdf:resource="http://www.w3.org/2000/01/rdf-schema#Property"/>
  </rdf:Description>
  <rdf:Description rdf:about="http://www.w3.org/ns/dcat#theme">
    <rdf:type rdf:resource="http://www.w3.org/2000/01/rdf-schema#Property"/>
  </rdf:Description>
  <rdf:Description rdf:about="http://www.w3.org/ns/dcat#downloadURL">
    <rdf:type rdf:resource="http://www.w3.org/2000/01/rdf-schema#Property"/>
  </rdf:Description>
  <rdf:Description rdf:about="http://dati.gov.it/onto/dcatapit#Dataset">
    <rdf:type rdf:resource="http://www.w3.org/2000/01/rdf-schema#Class"/>
  </rdf:Description>
  <rdf:Description rdf:about="https://w3id.org/italia/onto/CPSV/LifeEvent">
    <rdf:type rdf:resource="http://www.w3.org/2000/01/rdf-schema#Class"/>
  </rdf:Description>
  <rdf:Description rdf:about="https://w3id.org/italia/onto/CLV/hasRankOrder">
    <rdf:type rdf:resource="http://www.w3.org/2000/01/rdf-schema#Property"/>
  </rdf:Description>
  <rdf:Description rdf:about="http://www.w3.org/2004/02/skos/core#definition">
    <rdf:type rdf:resource="http://www.w3.org/2000/01/rdf-schema#Property"/>
  </rdf:Description>
  <rdf:Description rdf:about="http://www.w3.org/2006/vcard/ns#hasEmail">
    <rdf:type rdf:resource="http://www.w3.org/2000/01/rdf-schema#Property"/>
  </rdf:Description>
  <rdf:Description rdf:about="http://www.w3.org/2004/02/skos/core#inScheme">
    <rdf:type rdf:resource="http://www.w3.org/2000/01/rdf-schema#Property"/>
  </rdf:Description>
  <rdf:Description rdf:about="http://www.w3.org/ns/dcat#distribution">
    <rdf:type rdf:resource="http://www.w3.org/2000/01/rdf-schema#Property"/>
  </rdf:Description>
  <rdf:Description rdf:about="http://www.w3.org/ns/dcat#keyword">
    <rdf:type rdf:resource="http://www.w3.org/2000/01/rdf-schema#Property"/>
  </rdf:Description>
  <rdf:Description rdf:about="http://www.w3.org/2006/vcard/ns#Organization">
    <rdf:type rdf:resource="http://www.w3.org/2000/01/rdf-schema#Class"/>
  </rdf:Description>
  <rdf:Description rdf:about="http://www.w3.org/2006/vcard/ns#Kind">
    <rdf:type rdf:resource="http://www.w3.org/2000/01/rdf-schema#Class"/>
  </rdf:Description>
</rdf:RDF>
